fixed gcd (for real this time!)

trunk/source/LassoRanker/src/de/uni_freiburg/informatik/ultimate/plugins/analysis/lassoranker/Preferences.java
@@ -23,7 +23,7 @@ public class Preferences implements Serializable {
 	 * 
 	 * @see num_non_strict_invariants
 	 */
-	public static int num_strict_invariants = 0; // Default: 1
+	public static int num_strict_invariants = 1; // Default: 1
 	
 	/**
 	 * Number of non-strict supporting invariants for each Motzkin
@@ -36,7 +36,7 @@ public class Preferences implements Serializable {
 	 * 
 	 * @see num_strict_invariants
 	 */
-	public static int num_non_strict_invariants = 0; // Default: 1
+	public static int num_non_strict_invariants = 1; // Default: 1
 	
 	/**
 	 * Only consider non-decreasing invariants.
