trunk/examples/rank/Gcd_havoc.bpl
@@ -11,16 +11,16 @@ procedure main() returns (y1: int, y2: int)
   var y1_old: int;
   var y2_old: int;
   
-  assume(y1 >= 0);
-  assume(y2 >= 0);
+  assume(y1 >= 1);
+  assume(y2 >= 1);
   
-  while (y1 != y2) {
-    // if (y1 >= y2) then y1 := y1 - y2; else y2 := y2 - y1;
+  while (true) {
+    // if (y1 >= y2 + 1) then y1 := y1 - y2; else y2 := y2 - y1;
     y1_old := y1;
     y2_old := y2;
     havoc y1;
     havoc y2;
-    assume(y1_old < y2_old || y1 == y1_old - y2_old);
-    assume(y1_old >= y2_old || y2 == y2_old - y1_old);
+    assume((y1_old >= y2_old + 1 && y1 == y1_old - y2_old && y2 == y2_old)
+        || (y2_old >= y1_old + 1 && y2 == y2_old - y1_old && y1 == y1_old));
   }
 }
