trunk/examples/rank/Gcd.bpl
@@ -15,7 +15,7 @@ modifies y1, y2;
   assume(y1 >= 1);
   assume(y2 >= 1);
   while (y1 >= y2 + 1 || y2 >= y1 + 1) {
-    if (y1 > y2) {
+    if (y1 >= y2 + 1) {
       y1 := y1 - y2;
     } else {
       y2 := y2 - y1;
